updates

src/definitions.lean
@@ -23,7 +23,7 @@ inductive term : Type
 | and  : term → term → term
 | or   : term → term → term
 | imp  : term → term → term
-| elem : term → term → term
+| elem : type → term → term → term
 | pair : term → term → term
 | var  : ℕ → term
 | comp : type → term → term
@@ -37,16 +37,6 @@ open term
 -- * * * * * * * * * * * * * * * * * * * * * * * * * * * * * * * * * * * * * * * 
 
 instance nat_coe_var : has_coe ℕ term := ⟨term.var⟩
-
--- instance : has_zero term := ⟨term.var 0⟩
-
--- instance : has_one term := ⟨term.var 1⟩
-
--- def term_add : term → term → term
--- | (term.var n) (term.var m) := term.var (n+m)
--- | _ _ := star
-
--- instance : has_add term := ⟨term_add⟩
 
 @[simp] lemma var_simp {n : ℕ} : ↑n = (term.var n) := rfl
 
@@ -63,8 +53,7 @@ instance term_has_neg : has_neg term := ⟨not⟩
 def iff (p q: term) := (p ⟹ q) ⋀ (q ⟹ p)
 infix ` ⇔ `:60 := iff -- input \<=>
 
-infix ∈ := term.elem
-infix ∉ := λ a α, not (term.elem a α)
+notation a ` ∈[` A `] ` α := term.elem A a α
 notation `⟦ ` A ` | ` φ ` ⟧` := term.comp A φ
 
 notation `⟪` a `,` b `⟫` := term.pair a b 
@@ -83,14 +72,16 @@ def lift (d : ℕ) : ℕ → term → term
 | k (p ⋀ q)    := (lift k p) ⋀ (lift k q)
 | k (p ⋁ q)    := (lift k p) ⋁ (lift k q)
 | k (p ⟹ q)   := (lift k p) ⟹ (lift k q)
-| k (a ∈ α)    := (lift k a) ∈ (lift k α)
+| k (a ∈[A] α)    := (lift k a) ∈[A] (lift k α)
 | k ⟪a,b⟫      := ⟪lift k a, lift k b⟫
 | k (var m)    := if m≥k then var (m+d) else var m
 | k ⟦A | φ⟧  :=   ⟦A | lift (k+1) φ⟧
 | k (∀' A φ)   := ∀' A $ lift (k+1) φ
 | k (∃' A φ)   := ∃' A $ lift (k+1) φ
 
-prefix `^`:max := lift 1 0
+@[reducible]
+def lift_unit := lift 1 0
+prefix `^`:max := lift_unit
 
 section substitution
   variables {x p q a α b φ : term}
@@ -102,9 +93,9 @@ section substitution
   @[simp] lemma lift_and : ^(p ⋀ q) = ^p ⋀ ^q := rfl
   @[simp] lemma lift_or : ^(p ⋁ q) = ^p ⋁ ^q := rfl
   @[simp] lemma lift_imp : ^(p ⟹ q) = ^p ⟹ ^q := rfl
-  @[simp] lemma lift_elem : ^(a ∈ α) = (^a ∈ ^α) := rfl
+  @[simp] lemma lift_elem : ^(a ∈[A] α) = (^a ∈[A] ^α) := rfl
   @[simp] lemma lift_pair : ^(⟪a,b⟫) = ⟪^a,^b⟫ := rfl
-  @[simp] lemma lift_var {n : ℕ} : ^n = n.succ := rfl
+  @[simp] lemma lift_var {n : ℕ} : ^(term.var n) = term.var (n+1) := rfl
   
   @[simp] lemma lift_zero {k : ℕ} {a : term} : lift 0 k a = a :=
   by induction a generalizing k; simp *
@@ -128,7 +119,7 @@ section substitution
   | n x (p ⋀ q)    := (subst n x p) ⋀ (subst n x q)
   | n x (p ⋁ q)    := (subst n x p) ⋁ (subst n x q)
   | n x (p ⟹ q)  := (subst n x p) ⟹ (subst n x q)
-  | n x (a ∈ α)    := (subst n x a) ∈ (subst n x α)
+  | n x (a ∈[A] α)    := (subst n x a) ∈[A] (subst n x α)
   | n x ⟪a,b⟫      := ⟪subst n x a, subst n x b⟫
   | n x (var m)    := if n=m then x else if m > n then var (m-1) else var m
   | n x ⟦ A | φ ⟧   := ⟦A | subst (n+1) (^ x) φ⟧
@@ -187,7 +178,7 @@ section substitution
 
 end substitution
 
-def term_eq (A:type) (a₁ a₂ : term) : term := ∀' (𝒫 A) $ ((^ a₁) ∈ ↑0) ⇔ ((^ a₂) ∈ ↑0)
+def term_eq (A:type) (a₁ a₂ : term) : term := ∀' (𝒫 A) $ ((^ a₁) ∈[A] ↑0) ⇔ ((^ a₂) ∈[A] ↑0)
 notation a ` ≃[`:max A `] `:0 b := term_eq A a b
 
 @[simp] lemma subst_eq {A} {n x a₁ a₂} : subst n x (a₁ ≃[A] a₂) = a₁⁅x // n⁆ ≃[A] a₂⁅x // n⁆ := sorry
@@ -216,11 +207,11 @@ def ex_unique (A : type) (φ : term) : term :=
 prefix `∃!'`:2 := ex_unique
 
 def term_subset (A : type) (α : term) (β : term) : term :=
-  ∀' A $ (↑0 ∈ (^ α)) ⟹ (↑0 ∈ (^ β))
+  ∀' A $ (↑0 ∈[A] (^ α)) ⟹ (↑0 ∈[A] (^ β))
 notation a ` ⊆[`:max A `] `:0 b := term_subset A a b
 
 def term_prod (A B : type) (α β : term) : term :=
-  ⟦ A 𝕏 B | ∃[A,B] ((↑1 ∈ α) ⋀ (↑0 ∈ β) ⋀ (↑2 ≃[A 𝕏 B] ⟪↑1,↑0⟫))⟧
+  ⟦ A 𝕏 B | ∃[A,B] ((↑1 ∈[A] ^^^α) ⋀ (↑0 ∈[B] ^^^β) ⋀ (↑2 ≃[A 𝕏 B] ⟪↑1,↑0⟫))⟧
 
 -- * * * * * * * * * * * * * * * * * * * * * * * * * * * * * * * * * * * * * * *
 open list
@@ -236,7 +227,7 @@ inductive WF : context → type → term → Prop
 | and  {Γ p q}     : WF Γ Ω p → WF Γ Ω q → WF Γ Ω (p ⋀ q)
 | or   {Γ p q}     : WF Γ Ω p → WF Γ Ω q → WF Γ Ω (p ⋁ q)
 | imp  {Γ p q}     : WF Γ Ω p → WF Γ Ω q → WF Γ Ω (p ⟹ q)
-| elem {Γ A a α}   : WF Γ A a → WF Γ (𝒫 A) α → WF Γ Ω (a ∈ α)
+| elem {Γ A a α}   : WF Γ A a → WF Γ (𝒫 A) α → WF Γ Ω (a ∈[A] α)
 | pair {Γ A B a b} : WF Γ A a → WF Γ B b → WF Γ (A 𝕏 B) ⟪a,b⟫
 | var  {Γ A n}     : list.nth Γ n = some A → WF Γ A (var n)
 | comp {Γ A φ}     : WF (A::Γ) Ω φ → WF Γ (𝒫 A) ⟦A | φ⟧
@@ -265,13 +256,13 @@ inductive entails : context → term → term → Prop
 | all_intro  {Γ} {p φ A}   : entails (A::Γ) (^ p) φ → entails Γ p (∀' A φ)
 | ex_elim    {Γ} {p φ A}   : entails Γ (∃' A φ) p → entails (A::Γ) φ (^ p)
 | ex_intro   {Γ} {p φ A}   : entails (A::Γ) φ (^ p) → entails Γ (∃' A φ) p
-| extensionality {A}       : entails [] ⊤ $ ∀[𝒫 A, 𝒫 A] $ (∀' A $ (↑0 ∈ ↑2) ⇔ (↑0 ∈ ↑1)) ⟹ (↑1 ≃[𝒫 A] ↑0)
+| extensionality {A}       : entails [] ⊤ $ ∀[𝒫 A, 𝒫 A] $ (∀' A $ (↑0 ∈[A] ↑2) ⇔ (↑0 ∈[A] ↑1)) ⟹ (↑1 ≃[𝒫 A] ↑0)
 | prop_ext                 : entails [] ⊤ $ ∀[Ω,Ω] $ (↑1 ⇔ ↑0) ⟹ (↑1 ≃[Ω] ↑0)
 | star_unique              : entails [] ⊤ $ ∀[𝟙] (↑0 ≃[𝟙] ⁎)
 | pair_rep      {A B}      : entails [] ⊤ $ ∀[A 𝕏 B] $ ∃[A,B] $ ↑2 ≃[A 𝕏 B] ⟪↑1,↑0⟫
 | pair_distinct {A B}      : entails [] ⊤ $ ∀[A,B,A,B] $ (⟪↑3,↑2⟫ ≃[A 𝕏 B] ⟪↑1,↑0⟫) ⟹ ((↑3 ≃[A] ↑1) ⋀ (↑2 ≃[B] ↑0))
 | sub      {Γ} {p q b} (B) : WF Γ B b → entails (B::Γ) p q → entails Γ (p⁅b⁆) (q⁅b⁆)
-| comp     {Γ} {A φ}       : WF (A::Γ) Ω φ → entails Γ ⊤ (∀' A $ (↑0 ∈ (^ ⟦A | φ⟧)) ⇔ φ)
+| comp     {Γ} {A φ}       : WF (A::Γ) Ω φ → entails Γ ⊤ (∀' A $ (↑0 ∈[A] (^ ⟦A | φ⟧)) ⇔ φ)
 
 prefix `⊨`:1 := entails [] ⊤
 infix ` ⊨ `:50 := entails []
